Lab2: 4.2-4.6 implementation

LAB2/CircularBuffer.dfy
@@ -9,46 +9,112 @@ class CircularMemory
 
   constructor Init(cap : int) 
     requires cap > 0
-    requires cap <= MAX_INT
   {
-    cells := new int[cap];
+    // Initialize array cells with 0s
+    cells := new int[cap] (i => 0);
     read_position, write_position := 0, 0;
     isFlipped := false;
   }
-  predicate Valid() {...}
+
+  predicate Valid()
+    reads this
+  {
+    // There is nothing to read or write to if length isnt > 0
+    cells.Length > 0 &&
+    // Read and write can only have in-bounds indices (0 to cells.length - 1)
+    0 <= read_position < cells.Length &&
+    0 <= write_position < cells.Length
+  }
+
+  // A predicate indicating no more Read available
+  predicate isEmpty()
+    reads this
+  {
+    // This condition indicates the read pointer has read all available data and "caught up" to the writer
+    (read_position == write_position) && !isFlipped
+  }
+
+  // A predicate indicating no more Write should be allowed
+  predicate isFull()
+    reads this
+  {
+    // This condition indicates that the write pointer is about to "lap" the reader pointer
+    // and no further writing should be allowed to prevent loss of data
+    (read_position == write_position) && isFlipped
+  }
 
   method Read() returns (isSuccess : bool, content : int)
     modifies this
     requires Valid()
     ensures  Valid()
-    ensures  isSuccess ==> ...
-    ensures !isSuccess ==> ...
+    // When the read was successful, ensure the returned content is equal to
+    // what was stored in the cell which was read
+    ensures  isSuccess ==> (content == old(cells[read_position]))
+    // If there is no data to read (buffer was empty), ensure the dummy value 0 was returned
+    // and that the reading index remained unchanged
+    ensures !isSuccess ==> (content == 0) && (read_position == old(read_position))
 
   {
-    if(isFlipped)
+    // The case when there is no data to read
+    if (read_position == write_position) && !isFlipped
     {
-      ...
+      isSuccess := false;
+      content := 0;
     }
-    else // not flipped
+    // There is data to read
+    else
     {
-      ...
+      isSuccess := true;
+      content := cells[read_position];
+
+      // the case when read_position reached the end of the array and wraps to the beginning
+      if (read_position == cells.Length - 1)
+      {
+        read_position := 0;
+        isFlipped := !isFlipped;
+      }
+      else
+      {
+        read_position := read_position + 1;
+      }
     }
   }
 
+
   method Write(input : int) returns (isSuccess : bool)
-    modifies this
+    // The write method modifies object fields but also the cells array
+    modifies this, cells
     requires Valid()
     ensures  Valid()
-    ensures  isSuccess ==> ...
-    ensures !isSuccess ==> ...
+    // Ensure the cells array itself was not reassigned by the write method
+    ensures  cells == old(cells)
+    // When the write was successful, ensure the input value was stored
+    // in the cell which was written to
+    ensures  isSuccess ==> cells[old(write_position)] == input
+    // If the write failed (the buffer was full), ensure the write index remained unchanged
+    ensures !isSuccess ==> write_position == old(write_position)
   {
-    if(isFlipped)
+    // The case when the buffer is full and writing would overwrite existing data
+    if (read_position == write_position) && isFlipped
     {
-      ...
+      isSuccess := false;
     }
-    else // not flipped
+    else
     {
-      ...
+      isSuccess := true;
+
+      cells[write_position] := input;
+
+      // the case when write_position reached the end of the array and wraps to the beginning
+      if (write_position == cells.Length - 1)
+      {
+        write_position := 0;
+        isFlipped := !isFlipped;
+      }
+      else
+      {
+        write_position := write_position + 1;
+      }
     }
   }
 
